secure_api/merkle_tree/MerkleTree.Spec.fst
@@ -20,7 +20,8 @@ let hash_alg = Spec.Hash.Helpers.SHA2_256
 // - Spec.Hash.Helpers.size_hash_final_w SHA2_256 = 8
 // - Spec.Hash.Helpers.size_hash SHA2_256 = 32
 val hash_size: nat
-let hash_size = Spec.Hash.Helpers.size_hash hash_alg
+// joonwonc: KreMLin can't extract `Spec.Hash.Helpers.size_hash hash_alg`
+let hash_size = 32 
 
 // fournet: [tag] is a better name than [hash] for this
 // Thus `hash_raw` is bytes of length 32
